proofs/hol_light/aarch64/proofs/dump_bytecode.ml
@@ -6,28 +6,28 @@
 (* Load base theories for AArch64 from s2n-bignum *)
 needs "s2n_bignum/arm/proofs/base.ml";;
 
-print_string "=== bytecode start: aarch64/mldsa/mldsa_ntt.o ===\n";;
-print_literal_from_elf "aarch64/mldsa/mldsa_ntt.o";;
+print_string "=== bytecode start: aarch64/mldsa/ntt_aarch64_asm.o ===\n";;
+print_literal_from_elf "aarch64/mldsa/ntt_aarch64_asm.o";;
 print_string "==== bytecode end =====================================\n\n";;
 
-print_string "=== bytecode start: aarch64/mldsa/mldsa_pointwise.o ===\n";;
-print_literal_from_elf "aarch64/mldsa/mldsa_pointwise.o";;
+print_string "=== bytecode start: aarch64/mldsa/pointwise_montgomery_aarch64_asm.o ===\n";;
+print_literal_from_elf "aarch64/mldsa/pointwise_montgomery_aarch64_asm.o";;
 print_string "==== bytecode end =====================================\n\n";;
 
-print_string "=== bytecode start: aarch64/mldsa/mldsa_pointwise_acc_l4.o ===\n";;
-print_literal_from_elf "aarch64/mldsa/mldsa_pointwise_acc_l4.o";;
+print_string "=== bytecode start: aarch64/mldsa/mld_polyvecl_pointwise_acc_montgomery_l4_aarch64_asm.o ===\n";;
+print_literal_from_elf "aarch64/mldsa/mld_polyvecl_pointwise_acc_montgomery_l4_aarch64_asm.o";;
 print_string "==== bytecode end =====================================\n\n";;
 
-print_string "=== bytecode start: aarch64/mldsa/mldsa_pointwise_acc_l5.o ===\n";;
-print_literal_from_elf "aarch64/mldsa/mldsa_pointwise_acc_l5.o";;
+print_string "=== bytecode start: aarch64/mldsa/mld_polyvecl_pointwise_acc_montgomery_l5_aarch64_asm.o ===\n";;
+print_literal_from_elf "aarch64/mldsa/mld_polyvecl_pointwise_acc_montgomery_l5_aarch64_asm.o";;
 print_string "==== bytecode end =====================================\n\n";;
 
-print_string "=== bytecode start: aarch64/mldsa/mldsa_pointwise_acc_l7.o ===\n";;
-print_literal_from_elf "aarch64/mldsa/mldsa_pointwise_acc_l7.o";;
+print_string "=== bytecode start: aarch64/mldsa/mld_polyvecl_pointwise_acc_montgomery_l7_aarch64_asm.o ===\n";;
+print_literal_from_elf "aarch64/mldsa/mld_polyvecl_pointwise_acc_montgomery_l7_aarch64_asm.o";;
 print_string "==== bytecode end =====================================\n\n";;
 
-print_string "=== bytecode start: aarch64/mldsa/mldsa_poly_caddq.o ===\n";;
-print_literal_from_elf "aarch64/mldsa/mldsa_poly_caddq.o";;
+print_string "=== bytecode start: aarch64/mldsa/poly_caddq_aarch64_asm.o ===\n";;
+print_literal_from_elf "aarch64/mldsa/poly_caddq_aarch64_asm.o";;
 print_string "==== bytecode end =====================================\n\n";;
 
 print_string "=== bytecode start: aarch64/mldsa/poly_use_hint_32_aarch64_asm.o ===\n";;
@@ -38,8 +38,8 @@ print_string "=== bytecode start: aarch64/mldsa/poly_use_hint_88_aarch64_asm.o =
 print_literal_from_elf "aarch64/mldsa/poly_use_hint_88_aarch64_asm.o";;
 print_string "==== bytecode end =====================================\n\n";;
 
-print_string "=== bytecode start: aarch64/mldsa/mldsa_poly_chknorm.o ===\n";;
-print_literal_from_elf "aarch64/mldsa/mldsa_poly_chknorm.o";;
+print_string "=== bytecode start: aarch64/mldsa/poly_chknorm_aarch64_asm.o ===\n";;
+print_literal_from_elf "aarch64/mldsa/poly_chknorm_aarch64_asm.o";;
 print_string "==== bytecode end =====================================\n\n";;
 
 print_string "=== bytecode start: aarch64/mldsa/poly_decompose_32_aarch64_asm.o ===\n";;
@@ -50,10 +50,10 @@ print_string "=== bytecode start: aarch64/mldsa/poly_decompose_88_aarch64_asm.o 
 print_literal_from_elf "aarch64/mldsa/poly_decompose_88_aarch64_asm.o";;
 print_string "==== bytecode end =====================================\n\n";;
 
-print_string "=== bytecode start: aarch64/mldsa/mldsa_polyz_unpack_17.o ===\n";;
-print_literal_from_elf "aarch64/mldsa/mldsa_polyz_unpack_17.o";;
+print_string "=== bytecode start: aarch64/mldsa/polyz_unpack_17_aarch64_asm.o ===\n";;
+print_literal_from_elf "aarch64/mldsa/polyz_unpack_17_aarch64_asm.o";;
 print_string "==== bytecode end =====================================\n\n";;
 
-print_string "=== bytecode start: aarch64/mldsa/mldsa_polyz_unpack_19.o ===\n";;
-print_literal_from_elf "aarch64/mldsa/mldsa_polyz_unpack_19.o";;
+print_string "=== bytecode start: aarch64/mldsa/polyz_unpack_19_aarch64_asm.o ===\n";;
+print_literal_from_elf "aarch64/mldsa/polyz_unpack_19_aarch64_asm.o";;
 print_string "==== bytecode end =====================================\n\n";;
