proofs/hol_light/x86_64/proofs/dump_bytecode.ml
@@ -5,34 +5,34 @@
 
 needs "s2n_bignum/x86/proofs/base.ml";;
 
-print_string "=== bytecode start: x86_64/mldsa/mldsa_ntt.o ================\n";;
-print_literal_from_elf "x86_64/mldsa/mldsa_ntt.o";;
+print_string "=== bytecode start: x86_64/mldsa/ntt_avx2_asm.o ================\n";;
+print_literal_from_elf "x86_64/mldsa/ntt_avx2_asm.o";;
 print_string "==== bytecode end =====================================\n\n";;
 
-print_string "=== bytecode start: x86_64/mldsa/mldsa_intt.o ================\n";;
-print_literal_from_elf "x86_64/mldsa/mldsa_intt.o";;
+print_string "=== bytecode start: x86_64/mldsa/intt_avx2_asm.o ================\n";;
+print_literal_from_elf "x86_64/mldsa/intt_avx2_asm.o";;
 print_string "==== bytecode end =====================================\n\n";;
 
-print_string "=== bytecode start: x86_64/mldsa/mldsa_nttunpack.o ================\n";;
-print_literal_from_elf "x86_64/mldsa/mldsa_nttunpack.o";;
+print_string "=== bytecode start: x86_64/mldsa/nttunpack_avx2_asm.o ================\n";;
+print_literal_from_elf "x86_64/mldsa/nttunpack_avx2_asm.o";;
 print_string "==== bytecode end =====================================\n\n";;
 
-print_string "=== bytecode start: x86_64/mldsa/mldsa_pointwise.o ================\n";;
-print_literal_from_elf "x86_64/mldsa/mldsa_pointwise.o";;
+print_string "=== bytecode start: x86_64/mldsa/pointwise_avx2_asm.o ================\n";;
+print_literal_from_elf "x86_64/mldsa/pointwise_avx2_asm.o";;
 print_string "==== bytecode end =====================================\n\n";;
 
-print_string "=== bytecode start: x86_64/mldsa/mldsa_pointwise_acc_l4.o ================\n";;
-print_literal_from_elf "x86_64/mldsa/mldsa_pointwise_acc_l4.o";;
+print_string "=== bytecode start: x86_64/mldsa/pointwise_acc_l4_avx2_asm.o ================\n";;
+print_literal_from_elf "x86_64/mldsa/pointwise_acc_l4_avx2_asm.o";;
 print_string "==== bytecode end =====================================\n\n";;
 
-print_string "=== bytecode start: x86_64/mldsa/mldsa_pointwise_acc_l5.o ================\n";;
-print_literal_from_elf "x86_64/mldsa/mldsa_pointwise_acc_l5.o";;
+print_string "=== bytecode start: x86_64/mldsa/pointwise_acc_l5_avx2_asm.o ================\n";;
+print_literal_from_elf "x86_64/mldsa/pointwise_acc_l5_avx2_asm.o";;
 print_string "==== bytecode end =====================================\n\n";;
 
-print_string "=== bytecode start: x86_64/mldsa/mldsa_pointwise_acc_l7.o ================\n";;
-print_literal_from_elf "x86_64/mldsa/mldsa_pointwise_acc_l7.o";;
+print_string "=== bytecode start: x86_64/mldsa/pointwise_acc_l7_avx2_asm.o ================\n";;
+print_literal_from_elf "x86_64/mldsa/pointwise_acc_l7_avx2_asm.o";;
 print_string "==== bytecode end =====================================\n\n";;
 
-print_string "=== bytecode start: x86_64/mldsa/keccak_f1600_x4_avx2.o ================\n";;
-print_literal_from_elf "x86_64/mldsa/keccak_f1600_x4_avx2.o";;
+print_string "=== bytecode start: x86_64/mldsa/keccak_f1600_x4_avx2_asm.o ================\n";;
+print_literal_from_elf "x86_64/mldsa/keccak_f1600_x4_avx2_asm.o";;
 print_string "==== bytecode end =====================================\n\n";;
