proofs/hol_light/aarch64/proofs/poly_chknorm_aarch64_asm.ml
@@ -13,10 +13,10 @@
 needs "s2n_bignum/arm/proofs/base.ml";;
 needs "mldsa_native/aarch64/proofs/aarch64_utils.ml";;
 
-(**** print_literal_from_elf "aarch64/mldsa/mldsa_poly_chknorm.o";;
+(**** print_literal_from_elf "aarch64/mldsa/poly_chknorm_aarch64_asm.o";;
  ****)
 
-let mldsa_poly_chknorm_mc = define_assert_from_elf "mldsa_poly_chknorm_mc" "aarch64/mldsa/mldsa_poly_chknorm.o"
+let mldsa_poly_chknorm_mc = define_assert_from_elf "mldsa_poly_chknorm_mc" "aarch64/mldsa/poly_chknorm_aarch64_asm.o"
 (*** BYTECODE START ***)
 [
   0x4e040c34;       (* arm_DUP_GEN Q20 X1 32 128 *)
