proofs/hol_light/README.md
@@ -53,22 +53,22 @@ echo '1+1;;' | nc -w 5 127.0.0.1 2012
 
 ### AArch64
 - ML-DSA Arithmetic:
-  * AArch64 poly_caddq: [mldsa_poly_caddq.S](aarch64/mldsa/mldsa_poly_caddq.S)
-  * AArch64 poly_chknorm: [mldsa_poly_chknorm.S](aarch64/mldsa/mldsa_poly_chknorm.S)
+  * AArch64 poly_caddq: [poly_caddq_aarch64_asm.S](aarch64/mldsa/poly_caddq_aarch64_asm.S)
+  * AArch64 poly_chknorm: [poly_chknorm_aarch64_asm.S](aarch64/mldsa/poly_chknorm_aarch64_asm.S)
   * AArch64 poly_use_hint (l=5,7): [poly_use_hint_32_aarch64_asm.S](aarch64/mldsa/poly_use_hint_32_aarch64_asm.S)
   * AArch64 poly_use_hint (l=4): [poly_use_hint_88_aarch64_asm.S](aarch64/mldsa/poly_use_hint_88_aarch64_asm.S)
   * AArch64 poly_decompose (l=5,7): [poly_decompose_32_aarch64_asm.S](aarch64/mldsa/poly_decompose_32_aarch64_asm.S)
   * AArch64 poly_decompose (l=4): [poly_decompose_88_aarch64_asm.S](aarch64/mldsa/poly_decompose_88_aarch64_asm.S)
-  * AArch64 pointwise multiplication: [mldsa_pointwise.S](aarch64/mldsa/mldsa_pointwise.S)
-  * AArch64 pointwise multiplication-accumulation (l=4): [mldsa_pointwise_acc_l4.S](aarch64/mldsa/mldsa_pointwise_acc_l4.S)
-  * AArch64 pointwise multiplication-accumulation (l=5): [mldsa_pointwise_acc_l5.S](aarch64/mldsa/mldsa_pointwise_acc_l5.S)
-  * AArch64 pointwise multiplication-accumulation (l=7): [mldsa_pointwise_acc_l7.S](aarch64/mldsa/mldsa_pointwise_acc_l7.S)
+  * AArch64 pointwise multiplication: [pointwise_montgomery_aarch64_asm.S](aarch64/mldsa/pointwise_montgomery_aarch64_asm.S)
+  * AArch64 pointwise multiplication-accumulation (l=4): [mld_polyvecl_pointwise_acc_montgomery_l4_aarch64_asm.S](aarch64/mldsa/mld_polyvecl_pointwise_acc_montgomery_l4_aarch64_asm.S)
+  * AArch64 pointwise multiplication-accumulation (l=5): [mld_polyvecl_pointwise_acc_montgomery_l5_aarch64_asm.S](aarch64/mldsa/mld_polyvecl_pointwise_acc_montgomery_l5_aarch64_asm.S)
+  * AArch64 pointwise multiplication-accumulation (l=7): [mld_polyvecl_pointwise_acc_montgomery_l7_aarch64_asm.S](aarch64/mldsa/mld_polyvecl_pointwise_acc_montgomery_l7_aarch64_asm.S)
 - FIPS202:
-  * Keccak-F1600 using lazy rotations[^HYBRID]: [keccak_f1600_x1_scalar.S](aarch64/mldsa/keccak_f1600_x1_scalar.S)
-  * Keccak-F1600 using v8.4-A SHA3 instructions: [keccak_f1600_x1_v84a.S](aarch64/mldsa/keccak_f1600_x1_v84a.S)
-  * 2-fold Keccak-F1600 using v8.4-A SHA3 instructions: [keccak_f1600_x2_v84a.S](aarch64/mldsa/keccak_f1600_x2_v84a.S)
-  * 'Hybrid' 4-fold Keccak-F1600 using scalar and v8-A Neon instructions: [keccak_f1600_x4_v8a_scalar.S](aarch64/mldsa/keccak_f1600_x4_v8a_scalar.S)
-  * 'Triple hybrid' 4-fold Keccak-F1600 using scalar, v8-A Neon and v8.4-A+SHA3 Neon instructions: [keccak_f1600_x4_v8a_v84a_scalar.S](aarch64/mldsa/keccak_f1600_x4_v8a_v84a_scalar.S)
+  * Keccak-F1600 using lazy rotations[^HYBRID]: [keccak_f1600_x1_scalar_aarch64_asm.S](aarch64/mldsa/keccak_f1600_x1_scalar_aarch64_asm.S)
+  * Keccak-F1600 using v8.4-A SHA3 instructions: [keccak_f1600_x1_v84a_aarch64_asm.S](aarch64/mldsa/keccak_f1600_x1_v84a_aarch64_asm.S)
+  * 2-fold Keccak-F1600 using v8.4-A SHA3 instructions: [keccak_f1600_x2_v84a_aarch64_asm.S](aarch64/mldsa/keccak_f1600_x2_v84a_aarch64_asm.S)
+  * 'Hybrid' 4-fold Keccak-F1600 using scalar and v8-A Neon instructions: [keccak_f1600_x4_v8a_scalar_hybrid_aarch64_asm.S](aarch64/mldsa/keccak_f1600_x4_v8a_scalar_hybrid_aarch64_asm.S)
+  * 'Triple hybrid' 4-fold Keccak-F1600 using scalar, v8-A Neon and v8.4-A+SHA3 Neon instructions: [keccak_f1600_x4_v8a_v84a_scalar_hybrid_aarch64_asm.S](aarch64/mldsa/keccak_f1600_x4_v8a_v84a_scalar_hybrid_aarch64_asm.S)
 
 
 
@@ -76,15 +76,15 @@ echo '1+1;;' | nc -w 5 127.0.0.1 2012
 
 
 - ML-DSA Arithmetic:
-  * x86_64 forward NTT: [mldsa_ntt.S](x86_64/mldsa/mldsa_ntt.S)
-  * x86_64 inverse NTT: [mldsa_intt.S](x86_64/mldsa/mldsa_intt.S)
-  * x86_64 NTT unpack: [mldsa_nttunpack.S](x86_64/mldsa/mldsa_nttunpack.S)
-  * x86_64 pointwise multiplication: [mldsa_pointwise.S](x86_64/mldsa/mldsa_pointwise.S)
-  * x86_64 pointwise multiplication-accumulation (l=4): [mldsa_pointwise_acc_l4.S](x86_64/mldsa/mldsa_pointwise_acc_l4.S)
-  * x86_64 pointwise multiplication-accumulation (l=5): [mldsa_pointwise_acc_l5.S](x86_64/mldsa/mldsa_pointwise_acc_l5.S)
-  * x86_64 pointwise multiplication-accumulation (l=7): [mldsa_pointwise_acc_l7.S](x86_64/mldsa/mldsa_pointwise_acc_l7.S)
+  * x86_64 forward NTT: [ntt_avx2_asm.S](x86_64/mldsa/ntt_avx2_asm.S)
+  * x86_64 inverse NTT: [intt_avx2_asm.S](x86_64/mldsa/intt_avx2_asm.S)
+  * x86_64 NTT unpack: [nttunpack_avx2_asm.S](x86_64/mldsa/nttunpack_avx2_asm.S)
+  * x86_64 pointwise multiplication: [pointwise_avx2_asm.S](x86_64/mldsa/pointwise_avx2_asm.S)
+  * x86_64 pointwise multiplication-accumulation (l=4): [pointwise_acc_l4_avx2_asm.S](x86_64/mldsa/pointwise_acc_l4_avx2_asm.S)
+  * x86_64 pointwise multiplication-accumulation (l=5): [pointwise_acc_l5_avx2_asm.S](x86_64/mldsa/pointwise_acc_l5_avx2_asm.S)
+  * x86_64 pointwise multiplication-accumulation (l=7): [pointwise_acc_l7_avx2_asm.S](x86_64/mldsa/pointwise_acc_l7_avx2_asm.S)
 - FIPS202:
-  * 4-fold Keccak-F1600 using AVX2: [keccak_f1600_x4_avx2.S](x86_64/mldsa/keccak_f1600_x4_avx2.S)
+  * 4-fold Keccak-F1600 using AVX2: [keccak_f1600_x4_avx2_asm.S](x86_64/mldsa/keccak_f1600_x4_avx2_asm.S)
 
 <!--- bibliography --->
 [^HYBRID]: Becker, Kannwischer: Hybrid scalar/vector implementations of Keccak and SPHINCS+ on AArch64, [https://eprint.iacr.org/2022/1243](https://eprint.iacr.org/2022/1243)
